src/QUIC.Impl.Header.Parse.fst
@@ -1,0 +1,94 @@
+module QUIC.Impl.Header.Parse
+
+open QUIC.Spec.Header.Parse
+open QUIC.Impl.Header.Base
+
+friend QUIC.Spec.Header.Parse
+
+module LP = LowParse.Low.Base
+module Public = QUIC.Impl.Header.Public
+module U8 = FStar.UInt8
+
+[@"opaque_to_smt"]
+let impl_short_protected_bits
+  (reserved_bits: secret_bitfield 2)
+  (key_phase: secret_bitfield 1)
+  (pnl: PN.packet_number_length_t)
+: Tot (x: Secret.uint8 { Secret.reveal x == mk_short_protected_bits (Secret.reveal reserved_bits) (Secret.v key_phase = 1) pnl })
+= Secret.set_bitfield #Secret.U8 (Secret.set_bitfield #Secret.U8 (Secret.set_bitfield #Secret.U8 (Secret.to_u8 0uy) 0ul 2ul (Secret.to_u8 pnl `Secret.sub` Secret.to_u8 1uy)) 2ul 3ul key_phase) 3ul 5ul reserved_bits
+
+[@"opaque_to_smt"]
+let impl_long_protected_bits
+  (reserved_bits: secret_bitfield 2)
+  (pnl: PN.packet_number_length_t)
+: Tot (x: Secret.uint8 { Secret.reveal x == mk_long_protected_bits (Secret.reveal reserved_bits) pnl })
+= Secret.set_bitfield #Secret.U8 (Secret.set_bitfield #Secret.U8 (Secret.to_u8 0uy) 0ul 2ul (Secret.to_u8 pnl `Secret.sub` Secret.to_u8 1uy)) 2ul 4ul reserved_bits
+
+let p_header
+  (h: header)
+: Tot Public.header
+= match h with
+  | BShort rb spin phase cid cid_len pnl ->
+    Public.PShort (impl_short_protected_bits rb phase pnl) spin cid cid_len
+  | BLong version dcid dcil scid scil spec ->
+    begin match spec with
+    | BInitial rb payload_and_pn_length pnl token token_length ->
+      Public.PLong (impl_long_protected_bits rb pnl) version dcid dcil scid scil (Public.PInitial payload_and_pn_length token token_length)
+    | BZeroRTT rb payload_and_pn_length pnl ->
+      Public.PLong (impl_long_protected_bits rb pnl) version dcid dcil scid scil (Public.PZeroRTT payload_and_pn_length)
+    | BHandshake rb payload_and_pn_length pnl ->
+      Public.PLong (impl_long_protected_bits rb pnl) version dcid dcil scid scil (Public.PHandshake payload_and_pn_length)
+    | BRetry unused odcid odcil ->
+      Public.PLong unused version dcid dcil scid scil (Public.PRetry odcid odcil)
+    end
+
+let public_header_len_correct
+  (h: header)
+: Lemma
+  (public_header_len h == Public.header_len (p_header h))
+= ()
+
+module Spec = QUIC.Spec.Header.Parse
+
+#push-options "--z3rlimit 1024 --query_stats"
+
+let public_g_header_p_header
+  (h: header)
+  (m: HS.mem)
+  (pn: PN.packet_number_t)
+: Lemma (
+    let gh = g_header h m pn in
+    let cid_len = dcid_len h in
+    let last = last_packet_number gh in
+    let (| ph, pn' |) = synth_header_recip cid_len last gh in
+    Public.g_header (p_header h) m == ph
+  )
+= ()
+
+#restart-solver
+
+let header_len_correct
+  h m pn
+=
+  allow_inversion header;
+  allow_inversion long_header_specifics;
+  let gh = g_header h m pn in
+  let cid_len = dcid_len h in
+  let last = last_packet_number gh in
+  let (| ph, pn' |) = synth_header_recip cid_len last gh in
+  public_g_header_p_header h m pn;
+  assert (Public.g_header (p_header h) m == ph);
+  serialize_header_eq cid_len last gh;
+  Public.header_len_correct cid_len m (p_header h);
+  public_header_len_correct h;
+  assert (Seq.length (LP.serialize (Public.serialize_header cid_len) ph) == U32.v (public_header_len h));
+  if is_retry h
+  then
+    assert (Secret.v (header_len h) == Spec.header_len (g_header h m pn))
+  else begin
+    assert (pn_offset gh + Secret.v (Spec.pn_length gh) == Spec.header_len gh);
+    assert (pn_offset gh == Seq.length (LP.serialize (Public.serialize_header cid_len) ph));
+    assert (Secret.v (header_len h) == Spec.header_len (g_header h m pn))
+  end
+
+#pop-options
