src/QUIC.Impl.Header.Parse.fsti
@@ -1,0 +1,17 @@
+module QUIC.Impl.Header.Parse
+open QUIC.Spec.Header.Parse
+include QUIC.Impl.Header.Base
+
+module HS = FStar.HyperStack
+module U32 = FStar.UInt32
+module Seq = FStar.Seq
+module PN = QUIC.Spec.PacketNumber.Base
+module Secret = QUIC.Secret.Int
+module Spec = QUIC.Spec.Header.Parse
+
+val header_len_correct
+  (h: header)
+  (m: HS.mem)
+  (pn: PN.packet_number_t)
+: Lemma
+  (Secret.v (header_len h) == Spec.header_len (g_header h m pn))
